servicer provider reworked and corrections as result

Protocol/Lib.fst
@@ -8,6 +8,15 @@ let ConcatList sep l = match l with
         if tl="" then hd
         else Concat (Concat hd sep) tl
 
+val ConcatTupleList: string -> list (string * string) -> string
+let ConcatTupleList sep l = match l with 
+  | [] -> ""
+  | (k,v)::tl -> 
+      let tl = ConcatTupleList sep tl in
+        if tl="" then Concatkv k "=" v
+        else 
+        (Concat (Concat (Concatkv k "=" v) sep) tl)
+
 val Concatkv: string -> string -> string -> string
 let Concatkv k sep v = 
 	let ks = Concat k sep in
@@ -25,6 +34,13 @@ let getStrInList l str = match l with
 	| hd::tl ->
 		if strStartsWith hd str then hd
 		else getStrInList tl str
+
+val getStrInTupleList: list (string*string) -> string -> string
+let getStrInTupleList l str = match l with
+	| [] -> ""
+	| (k,v)::tl ->
+		if k = str then v
+		else getStrInTupleList tl str
 
 val isEmptyStr: string -> bool
 let isEmptyStr str = match str with
