Protocol/Network.fst
@@ -19,14 +19,14 @@ extern Network val RecieveRequest: prin -> (string * string * string * list stri
 *)
 
 type HttpMessage =
-	| Get: prin -> string -> list string -> list string -> HttpMessage
- 	| Post: prin -> list string -> list string -> HttpMessage
- 	| Redirect: prin -> string -> list string -> list string -> HttpMessage
-	| Response: int -> body:string -> HttpMessage
+	| Get: prin -> string -> list (string * string) -> list (string * string) -> HttpMessage
+ 	| Post: prin -> list (string * string) -> list (string * string) -> HttpMessage
+ 	| Redirect: prin -> string -> list (string * string) -> list (string * string) -> HttpMessage
+	| Response: int -> body:string -> list (string * string) -> HttpMessage
 
-val buildDestination: string -> list string -> string
+val buildDestination: string -> list (string * string) -> string
 let buildDestination url params =
-	 let paramStr = ConcatList ";" params in
+	 let paramStr = ConcatTupleList ";" params in
 	 Concatkv url "?" paramStr
 
 val Send: HttpMessage -> unit
@@ -34,7 +34,8 @@ let Send message =
 	match message with
 	| Get (prin,url,params,cookies) -> 
 		let dest = buildDestination url params in
-		SendRequest dest cookies "hello";()
+		let cl = map (fun (k,v)-> Concatkv k "=" v) cookies in
+		SendRequest dest cl "hello";()
 	| _ -> println "Not yet implemented";
 		()
 
@@ -43,6 +44,7 @@ let Recieve client =
 	let (verb,url,body,cookies) = RecieveRequest client in
 	match verb with
 	| "GET" -> 
-		let params = ["here query=params should be"] in
-		Get client url params cookies
-	| _ -> Response 400 "failed"
+		let params = [("here query", "params should be")] in
+		let c = [("atemp","cookie")]
+in		Get client url params c
+	| _ -> Response 400 "failed" []
