Protocol/Saml.fst
@@ -16,15 +16,14 @@ extern reference Saml {language="F#";
             classname="Saml"}
 
 extern Saml val CreateAuthnRequest: issuer:prin -> destination:prin -> samlmessage
-extern Saml val CreateChallenge: prin -> nonce
 extern Saml val CreateSamlAssertion: user:string -> issuer:prin -> destination:prin -> assertion
 extern Saml val CreateSamlResponse: issuer:prin -> destination:prin -> assertion -> samlmessage
 extern Saml val CreateSamlFailedResponse: issuer:prin -> destination:prin -> SamlStatus -> samlmessage
 
-val CreateRedirectResponse: prin -> samlmessage -> dsig -> string -> HttpMessage
-let CreateRedirectResponse prin msg sig relay =
+val CreateRedirectResponse: prin -> samlmessage -> dsig -> HttpMessage
+let CreateRedirectResponse prin msg sig =
       (*Base64 encode all params*)
-      let params = [msg; sig; relay] in
-      let cookies = [relay] in
+      let params = [("samlmessage",msg); ("signature",sig)] in
+      let cookies = [] in
       let resp = Redirect prin prin params cookies in 
       resp
