Protocol/ServiceProvider.fst
@@ -1,26 +1,46 @@
 module Serviceprovider
+
+open Lib
+open ContentServer
 open Protocol
+open Saml
+open Crypto
+open Network
+
+val hasValidSession: list (string*string) -> bool
+let hasValidSession cookies = 
+  (* Find AuthenticationKey cookie and validate *)
+  let ak = getStrInTupleList cookies "AuthenticationKey" in
+  if isEmptyStr ak then false 
+  else true (*Should be validated somehow*)
 
 val serviceprovider:  me:prin -> pubkey me -> privkey me ->
                       browser:prin -> idp:prin -> pubkey idp -> unit 
 let serviceprovider me pubk privk browser idp pubkidp = 
   let reqRes = Recieve browser in (*1*) (*7*)
   match reqRes with
-  | HttpGet (uri) -> 
+  | Get (prin,uri,params,cookies) -> 
 
-    let authnReq = CreateAuthnRequest me idp in 
-    assume(Log me authnReq) (*Protocol event*);
-    let sigSP = Sign me privk authnReq in
-      
-    let authnReqest = SamlProtocolMessage idp authnReq sigSP in 
-    Send browser authnReqest (*2*)  
+    (*Check for valid session*)
+    if hasValidSession cookies then
+      let resp = Response 200 (getContent uri) [] in
+      Send resp (*8*)
+    else (*Create AuthnRequest and send (via client) to idp*)
+      (let authnReq = CreateAuthnRequest me idp in 
+      assume(Log me authnReq) (*Protocol event*);
+      let sigSP = Sign me privk authnReq in
+      let resp = CreateRedirectResponse idp authnReq sigSP in 
+      Send resp (*2*))
 
-  | SamlProtocolMessage (sp, msg, sigIDP) -> 
+  | Post (sp, params, cookies) -> 
+      let msg = getStrInTupleList params "SamlMessage" in
+      let sigIDP = getStrInTupleList params "Signature" in
       if VerifySignature idp pubkidp msg sigIDP
       then
         (assert(Log idp msg);
-          let resource = Resource "uri" in
-          Send browser resource)  (*8*)
-      else Send browser (Failed (403))(*8.1*)
+          let ak =  GenerateNonce sp in
+          let resp = Response 200 (getContent "Loggedin") [("AuthenticationKey", ak)] in
+          Send resp) (*8*)
+      else Send (Response 403 (getErrorPage 403) [])(*8.1*)
   
-  | _ -> Send browser (Failed (400))(*2.1*)
+  | _ -> Send (Response 400 (getErrorPage 400) [])
