Protocol/ContentServer.fst
@@ -1,0 +1,18 @@
+module ContentServer
+
+val buildErrorPage: string -> string
+let buildErrorPage msg =
+	let errorHeader = "<html><head><title>the page</title></head><body>" in
+	let errorFooter = "</body></html>" in
+	Concat errorHeader (Concat msg errorFooter)
+
+val getContent: string -> string
+let getContent page =
+	(*Should read the specified page and return it*)
+	"<html><head><title>the page</title></head><body>You are now logged in</body></html>"
+
+val getErrorPage: int -> string
+let getErrorPage status = match	status with
+	| 400 -> buildErrorPage "400 - Bad request"
+	| 403 -> buildErrorPage "403 - Forbidden"
+	| _ -> buildErrorPage "500 - internal server error"
